no_es_cl_ecca_tests.v
@@ -1,0 +1,57 @@
+Require Import no_es_cl_ecca.
+Require Import abstract_machine_facts.
+
+
+Module Sim := DetAbstractMachine_Sim ECCa_es_cl_EAM_minus.
+
+Import ECCa_es_cl_EAM_minus.
+Import no_es_cl_ECCa.
+Import no_es_cl_ECCa_Ref.R.
+
+
+
+Let t1 := Lam0 (App0 (Lam0 (Lam0 (Var0 1))) (Var0 0)).
+
+
+Eval compute in 
+    Sim.n_steps 
+    ( c_init t1 )
+    14.
+
+
+Eval compute in 
+    Sim.n_steps 
+    ( c_init (Lam0 (App0  t1  (Var0 0) )) )
+    20.
+
+
+
+Fixpoint nat_term0 n :=
+    match n with
+    | 0   => Lam0 (Lam0 (Var0 0))
+    | S n => Lam0 (Lam0 (App0 (Var0 1) (App0 (App0 (nat_term0 n) (Var0 1)) (Var0 0))))
+    end.
+
+
+Let add_term0 := 
+    Lam0 (Lam0 (Lam0 (Lam0 
+        (App0 (App0 (Var0 3) 
+            (Var0 1)) 
+            (App0 (App0 (Var0 2) (Var0 1)) (Var0 0)))))).
+
+Let mul_term0 := 
+    Lam0 (Lam0 (Lam0 (Lam0
+        (App0 (App0
+
+        (App0 (App0 (Var0 2) 
+            (Lam0 (App0 (App0 add_term0 (Var0 4)) (Var0 0)) ))
+            (nat_term0 0))
+
+        (Var0 1)) (Var0 0))))).
+
+
+Eval compute in
+    Sim.n_steps 
+    ( c_init (App0 (App0 mul_term0 (nat_term0 3)) (nat_term0 4)) ) 
+    672.
+
