refocusing_machine_sig.v
@@ -250,11 +250,15 @@ Module Type PROPER_EA_MACHINE (R : RED_LANG) (RS : RED_REF_SEM R) <: DET_ABSTRAC
 
 
   Reserved Notation "c1 →+ c2" (at level 40, no associativity).
+  Reserved Notation "c1 →* c2" (at level 40, no associativity).
 
   Inductive trans_close : configuration -> configuration -> Prop :=
   | one_step   : forall c1 c2,     c1 → c2  ->  c1 →+ c2
   | multi_step : forall c1 c2 c3,  c1 → c2  ->  c2 →+ c3  ->  c1 →+ c3
   where "c1 →+ c2" := (trans_close c1 c2).
+
+  Definition trans_ref_close c1 c2 := c1 = c2 \/ trans_close c1 c2.
+  Notation "c1 →* c2" := (trans_ref_close c1 c2).
 
 
   Inductive eval : term -> value -> Prop :=
@@ -401,11 +405,15 @@ Module Type PROPER_PE_MACHINE (R : RED_LANG) (PERS : PE_REF_SEM R) <: DET_ABSTRA
 
 
   Reserved Notation "c1 →+ c2" (at level 40, no associativity).
+  Reserved Notation "c1 →* c2" (at level 40, no associativity).
 
   Inductive trans_close : configuration -> configuration -> Prop :=
   | one_step   : forall c1 c2,     c1 → c2  ->  c1 →+ c2
   | multi_step : forall c1 c2 c3,  c1 → c2  ->  c2 →+ c3  ->  c1 →+ c3
   where "c1 →+ c2" := (trans_close c1 c2).
+
+  Definition trans_ref_close c1 c2 := c1 = c2 \/ trans_close c1 c2.
+  Notation "c1 →* c2" := (trans_ref_close c1 c2).
 
   Inductive eval : term -> value -> Prop :=
   | e_intro : forall t v, trans_close (c_init t) (c_final v) -> eval t v.
